use more efficient uleb128 encoding for nats

lib/Binary.v
@@ -113,3 +113,139 @@ Proof.
   apply binary_to_nat_to_binary_rec.
   apply le_refl.
 Qed.
+
+Fixpoint bits_of (n_bits : nat) (x : nat) : (list bool * nat) :=
+  match n_bits with
+  | 0 => ([], x)
+  | S n_bits' => let (l,x') := bits_of n_bits' (Nat.div2 x)
+                in (Nat.odd x :: l, x')
+  end.
+
+Lemma length_bits_of :
+  forall n x l x', bits_of n x = (l, x') ->
+              length l = n.
+Proof.
+  induction n; simpl; intros x l x' H.
+  - find_inversion. auto.
+  - break_let. apply IHn in Heqp.
+    find_inversion. auto.
+Qed.
+
+Fixpoint uleb128_encode' fuel n : list bool :=
+  let (byte, n') := bits_of 7 n
+  in match n' with
+     | 0 => false :: byte
+     | S _ => true :: byte ++
+             match fuel with
+             | 0 => []
+             | S fuel' => uleb128_encode' fuel' n'
+             end
+     end.
+Definition uleb128_encode n := uleb128_encode' n n.
+
+Fixpoint uleb128_decode (bin : list bool) : option (nat * list bool) :=
+  match bin with
+  | b_cont::b0::b1::b2::b3::b4::b5::b6::bin' =>
+    let n := binary_to_nat_rec [b0;b1;b2;b3;b4;b5;b6]
+    in if b_cont
+       then match uleb128_decode bin' with None => None
+            | Some (ans, bin'') => Some (n + 128 * ans, bin'')
+            end
+       else Some (n, bin')
+  | _ => None
+  end.
+
+Lemma shiftr_div2_comm :
+  forall b a,
+    Nat.shiftr (Nat.div2 a) b = Nat.div2 (Nat.shiftr a b).
+Proof.
+  induction b; simpl; intros a; auto using f_equal.
+Qed.
+
+Lemma bits_of_x' :
+  forall n x l x',
+    bits_of n x = (l, x') ->
+    x' = Nat.shiftr x n.
+Proof.
+  induction n; simpl; intros x l x' H.
+  - now find_inversion.
+  - break_let. apply IHn in Heqp. find_inversion. apply shiftr_div2_comm.
+Qed.
+
+Lemma mod2n_succ:
+  forall n x : nat, Nat.b2n (Nat.odd x) + 2 * (Nat.div2 x mod 2 ^ n) = x mod 2 ^ S n.
+Proof.
+  intros n x.
+  apply Nat.bits_inj.
+  intro i.
+  repeat rewrite <- Nat.land_ones.
+  repeat rewrite Nat.land_spec.
+  rewrite plus_comm.
+  destruct i.
+  + now rewrite Nat.testbit_0_r, Nat.ones_spec_low, Nat.bit0_odd, Bool.andb_true_r by omega.
+  + rewrite Nat.testbit_succ_r, Nat.land_spec, Nat.div2_spec, Nat.shiftr_specif, plus_comm.
+    f_equal.
+    destruct (lt_dec i n).
+    * now rewrite !Nat.ones_spec_low by omega.
+    * now rewrite !Nat.ones_spec_high by omega.
+Qed.
+
+Lemma bits_of_l :
+  forall n x l x',
+    bits_of n x = (l, x') ->
+    binary_to_nat_rec l = x mod (2 ^ n).
+Proof.
+  induction n; intros x l x' H.
+  - simpl in *. now find_inversion.
+  - cbn [bits_of] in *.
+    break_let. apply IHn in Heqp.
+    find_inversion.
+    cbn [binary_to_nat_rec].
+    rewrite Heqp.
+    apply mod2n_succ.
+Qed.
+
+Lemma bits_of_reconstruct :
+  forall n x l x',
+    bits_of n x = (l, x') ->
+    x = binary_to_nat_rec l + 2 ^ n * x'.
+Proof.
+  intros.
+  find_copy_apply_lem_hyp bits_of_l.
+  find_apply_lem_hyp bits_of_x'.
+  subst.
+  now rewrite Nat.shiftr_div_pow2, H0, plus_comm, <- Nat.div_mod
+    by (apply Nat.pow_nonzero; congruence).
+Qed.
+
+Lemma uleb128_decode_encode' :
+  forall fuel n bin,
+    n <= fuel ->
+    uleb128_decode (uleb128_encode' fuel n ++ bin) = Some (n, bin).
+Proof.
+  induction fuel as [|fuel' IHfuel']; intros n bin Hle.
+  - destruct n.
+    + reflexivity.
+    + omega.
+  - cbn [uleb128_encode'].
+    break_let.
+    find_copy_apply_lem_hyp length_bits_of.
+    do 8 (destruct l; simpl in H; try omega).
+    find_apply_lem_hyp bits_of_reconstruct.
+    subst n.
+    break_match; cbn [app uleb128_decode].
+    + f_equal. f_equal. omega.
+    + rewrite IHfuel'; auto.
+      replace (2 ^ 7) with 128 in * by auto.
+      omega.
+Qed.
+
+Lemma uleb128_decode_encode :
+  forall n bin,
+    uleb128_decode (uleb128_encode n ++ bin) = Some (n, bin).
+Proof.
+  unfold uleb128_encode.
+  intros.
+  apply uleb128_decode_encode'.
+  auto.
+Qed.
